tools/local-dafny.sh
@@ -7,7 +7,7 @@
 echo "NOTE: using /noNLarith and /compile:0"
 DIR="$( cd "$( dirname "${BASH_SOURCE[0]}" )" >/dev/null 2>&1 && pwd )"
 #set -x
-cmd="$DIR/../.dafny/bin/dafny $@ /induction:1 /noNLarith /compile:0 /timeLimit:20"
+cmd="$DIR/../.dafny/bin/dafny $@ /induction:1 /noNLarith /compile:0 /rlimit:16350"
 # if you don't have unbuffer, apt-get install expect
 # unbuffer convinces dafny to emit colored errors even when stdout is a pipe.
 # stdbuf -o0 and --line-buffered are my belt-and-suspenders attempts to keep dafny
